coq/CoqOfSolidity/proofs/CoqOfSolidity.v
@@ -1,0 +1,394 @@
+Require Import CoqOfSolidity.CoqOfSolidity.
+Require Import simulations.CoqOfSolidity.
+
+Import RunO.
+
+Module Memory.
+  Definition of_u256_list (words : list U256.t) : Memory.t.
+  Admitted.
+
+  Lemma run_mload codes environment state
+      (words : list U256.t) (index : nat) (word : U256.t) :
+    List.nth_error words index = Some word ->
+    state.(State.memory) = of_u256_list words ->
+    {{? codes, environment, Some state |
+      Stdlib.mload (32 * Z.of_nat index) ⇓
+      Result.Ok word
+    | Some state ?}}.
+  Proof.
+  Admitted.
+
+  Lemma run_mstore codes environment state
+      (words : list U256.t) (index : nat) (word : U256.t) :
+    match List.update_nth words index word with
+    | Some words' =>
+      let state' := state <| State.memory := of_u256_list words' |> in
+      {{? codes, environment, Some state |
+        Stdlib.mstore (32 * Z.of_nat index) word ⇓
+        Result.Ok tt
+      | Some state' ?}}
+    | None => True
+    end.
+  Proof.
+  Admitted.
+End Memory.
+
+Module SimulatedMemory.
+  Definition t : Set :=
+    list U256.t.
+
+  Definition init : t :=
+    [0; 0; 0; 0; 0].
+End SimulatedMemory.
+
+Module Address.
+  Lemma implies_and_mask address :
+    Address.Valid.t address ->
+    address = Z.land address (2 ^ 160 - 1).
+  Proof.
+  Admitted.
+End Address.
+
+(** A value that admits a direct representation on the storage. *)
+Module StorableValue.
+  (** For now the maps can only contain integers. *)
+  Inductive t : Set :=
+  | U256 (value : U256.t)
+  | Map (value : Dict.t U256.t U256.t)
+  | Map2 (value : Dict.t (U256.t * U256.t) U256.t).
+
+  (** The default value is zero when a key is not yet assigned. *)
+  Definition map_get_u256 {K : Set} `{Dict.Eq.C K}
+      (map : Dict.t K U256.t) (key : K) : U256.t :=
+    match Dict.get map key with
+    | Some value => value
+    | None => 0
+    end.
+
+  Lemma map_get_u256_is_valid {K : Set} `{Dict.Eq.C K} (P_K : K -> Prop)
+      (map : Dict.t K U256.t) (key : K)
+      (H_map : Dict.Valid.t P_K U256.Valid.t map) :
+    U256.Valid.t (map_get_u256 map key).
+  Proof.
+    unfold map_get_u256.
+    pose proof (Dict.get_is_valid _ _ _ key H_map).
+    destruct Dict.get; unfold U256.Valid.t in *; lia.
+  Qed.
+End StorableValue.
+
+Module IsStorable.
+  Class C (A : Set) : Set := {
+    to_storable_value : A -> StorableValue.t;
+  }.
+
+  Global Instance IU256 : C U256.t := {
+    to_storable_value := StorableValue.U256;
+  }.
+
+  Global Instance IMap : C (Dict.t U256.t U256.t) := {
+    to_storable_value := StorableValue.Map;
+  }.
+
+  Global Instance IMap2 : C (Dict.t (U256.t * U256.t) U256.t) := {
+    to_storable_value := StorableValue.Map2;
+  }.
+End IsStorable.
+
+Module State.
+  Definition get_current_storage
+      (environment : Environment.t) (state : State.t) :
+      option Storage.t :=
+    let address := environment.(Environment.address) in
+    let account := Dict.get state.(State.accounts) address in
+    match account with
+    | None => None
+    | Some account => Some account.(Account.storage)
+    end.
+
+  Definition with_current_storage
+      (environment : Environment.t) (state : State.t) (storage : Storage.t) :
+      State.t :=
+    let address := environment.(Environment.address) in
+    let accounts :=
+      Dict.assign_function state.(State.accounts) address (fun account =>
+        account <| Account.storage := storage |>
+      ) in
+    match accounts with
+    | None => state
+    | Some accounts => state <| State.accounts := accounts |>
+    end.
+
+  Lemma get_current_storage_with_current_storage_eq
+      environment state storage :
+    get_current_storage environment (with_current_storage environment state storage) =
+    Some storage.
+  Proof.
+  Admitted.
+End State.
+Global Opaque State.get_current_storage State.with_current_storage.
+
+Lemma run_keccak256_tuple2 codes environment state
+    (memory : list U256.t) (index : nat) (a b : U256.t) :
+  state.(State.memory) = Memory.of_u256_list memory ->
+  List.nth_error memory index = Some a ->
+  List.nth_error memory (S index) = Some b ->
+  {{? codes, environment, Some state |
+    Stdlib.keccak256 (32 * (Z.of_nat index)) (32 * 2) ⇓
+    Result.Ok (keccak256_tuple2 a b)
+  | Some state ?}}.
+Proof.
+Admitted.
+
+Module Storage.
+  Definition of_storable_values (values : list StorableValue.t) : Storage.t.
+  Admitted.
+
+  Lemma run_sload_u256
+      (values : list StorableValue.t)
+      (index : nat)
+      (value : U256.t)
+      codes environment state :
+    State.get_current_storage environment state = Some (of_storable_values values) ->
+    List.nth_error values index = Some (StorableValue.U256 value) ->
+    {{? codes, environment, Some state |
+      Stdlib.sload (Z.of_nat index) ⇓
+      Result.Ok value
+    | Some state ?}}.
+  Proof.
+  Admitted.
+
+  Lemma run_sstore_u256
+      (values : list StorableValue.t)
+      (index : nat)
+      (value : U256.t)
+      codes environment state :
+    let state := State.with_current_storage environment state (of_storable_values values) in
+    match List.update_nth values index (StorableValue.U256 value) with
+    | Some values' =>
+      let state' := State.with_current_storage environment state (of_storable_values values') in
+      {{? codes, environment, Some state |
+        Stdlib.sstore (Z.of_nat index) value ⇓
+        Result.Ok tt
+      | Some state' ?}}
+    | None => True
+    end.
+  Proof.
+  Admitted.
+
+  Lemma run_sload_map_u256
+      (values : list StorableValue.t)
+      (index : nat)
+      (map : Dict.t U256.t U256.t)
+      (key : U256.t)
+      codes environment state :
+    List.nth_error values index = Some (StorableValue.Map map) ->
+    {{? codes, environment, state |
+      Stdlib.sload (keccak256_tuple2 key (Z.of_nat index)) ⇓
+      Result.Ok (StorableValue.map_get_u256 map key)
+    | state ?}}.
+  Proof.
+  Admitted.
+
+  Lemma run_sstore_map_u256
+      (values : list StorableValue.t)
+      (index : nat)
+      (key : U256.t) (value : U256.t)
+      codes environment state :
+    State.get_current_storage environment state = Some (of_storable_values values) ->
+    match List.nth_error values index with
+    | Some (StorableValue.Map map) =>
+      let map' := Dict.declare_or_assign map key value in
+      match List.update_nth values index (StorableValue.Map map') with
+      | Some values' =>
+        let state' := State.with_current_storage environment state (of_storable_values values') in
+        {{? codes, environment, Some state |
+          Stdlib.sstore (keccak256_tuple2 key (Z.of_nat index)) value ⇓
+          Result.Ok tt
+        | Some state' ?}}
+      | None => True
+      end
+    | _ => True
+    end.
+  Proof.
+  Admitted.
+
+  Lemma run_sload_map2_u256
+      (values : list StorableValue.t)
+      (index : nat)
+      (map : Dict.t (U256.t * U256.t) U256.t)
+      (key1 key2 : U256.t)
+      codes environment state :
+    List.nth_error values index = Some (StorableValue.Map2 map) ->
+    {{? codes, environment, state |
+      Stdlib.sload (keccak256_tuple2 key2 (keccak256_tuple2 key1 (Z.of_nat index))) ⇓
+      Result.Ok (StorableValue.map_get_u256 map (key1, key2))
+    | state ?}}.
+  Proof.
+  Admitted.
+
+  Lemma run_sstore_map2_u256
+      (values : list StorableValue.t)
+      (index : nat)
+      (key1 key2 : U256.t) (value : U256.t)
+      codes environment state :
+    State.get_current_storage environment state = Some (of_storable_values values) ->
+    match List.nth_error values index with
+    | Some (StorableValue.Map2 map) =>
+      let map' := Dict.declare_or_assign map (key1, key2) value in
+      match List.update_nth values index (StorableValue.Map2 map') with
+      | Some values' =>
+        let state' := State.with_current_storage environment state (of_storable_values values') in
+        {{? codes, environment, Some state |
+          Stdlib.sstore
+            (keccak256_tuple2 key2 (keccak256_tuple2 key1 (Z.of_nat index))) value ⇓
+          Result.Ok tt
+        | Some state' ?}}
+      | None => True
+      end
+    | _ => True
+    end.
+  Proof.
+  Admitted.
+End Storage.
+
+Module SimulatedStorage.
+  Definition t : Set :=
+    list StorableValue.t.
+
+  Definition init : t := [
+    StorableValue.Map [];
+    StorableValue.Map [];
+    StorableValue.U256 0
+  ].
+End SimulatedStorage.
+
+Definition make_state environment state
+    (memory : SimulatedMemory.t) (storage : SimulatedStorage.t) :
+    State.t :=
+  State.with_current_storage environment
+    (state <| State.memory := Memory.of_u256_list memory |>)
+    (Storage.of_storable_values storage).
+
+Lemma get_memory_make_state_eq environment state
+    memory storage :
+  (make_state environment state memory storage).(State.memory) =
+  Memory.of_u256_list memory.
+Proof.
+Admitted.
+
+(** Lemma to put the state always in the same form. *)
+Module CanonizeState.
+  Lemma update_memory_eq environment state
+      memory storage new_memory :
+    (make_state environment state memory storage) <|
+      State.memory := Memory.of_u256_list new_memory
+    |> =
+    make_state environment state new_memory storage.
+  Proof.
+  Admitted.
+
+  Lemma update_storage_eq environment state
+        memory storage new_storage :
+    State.with_current_storage environment
+      (make_state environment state memory storage)
+      (Storage.of_storable_values new_storage) =
+    make_state environment state memory new_storage.
+  Proof.
+  Admitted.
+
+  Lemma with_current_storage_twice_eq environment state
+      storage1 storage2 :
+    State.with_current_storage environment
+      (State.with_current_storage environment state storage1)
+      storage2 =
+    State.with_current_storage environment state storage2.
+  Proof.
+  Admitted.
+
+  Ltac execute := repeat (
+    rewrite update_memory_eq ||
+    rewrite update_storage_eq ||
+    rewrite with_current_storage_twice_eq ||
+    match goal with
+    | |- context[
+      State.with_current_storage ?environment
+        (?state <|State.memory:= Memory.of_u256_list ?memory |>)
+        (Storage.of_storable_values ?storage)
+      ] => fold (make_state environment state memory storage)
+    end
+  ).
+End CanonizeState.
+
+Ltac apply_run_mload :=
+  match goal with
+  | |- {{? _, _, Some (make_state _ _ ?memory _) | Stdlib.mload ?offset ⇓ _ | _ ?}} =>
+    eapply (Memory.run_mload _ _ _ memory (Z.to_nat (offset / 32)));
+    try reflexivity;
+    try apply get_memory_make_state_eq
+  end.
+
+Ltac apply_run_mstore :=
+  match goal with
+  | |- {{? _, _, Some (make_state _ _ ?memory _) | Stdlib.mstore ?offset ?value ⇓ _ | _ ?}} =>
+    apply (Memory.run_mstore _ _ _ memory (Z.to_nat (offset / 32)) value)
+  end.
+
+Ltac apply_run_sload_u256 :=
+  match goal with
+  | |- {{? _, _, Some (make_state _ _ _ ?storage) | Stdlib.sload ?slot ⇓ _ | _ ?}} =>
+    apply (Storage.run_sload_u256 storage (Z.to_nat slot));
+    try reflexivity;
+    try apply State.get_current_storage_with_current_storage_eq
+  end.
+
+Ltac apply_run_sstore_u256 :=
+  match goal with
+  | |- {{? _, _, Some (make_state _ _ _ ?storage) | Stdlib.sstore ?slot ?value ⇓ _ | _ ?}} =>
+    apply (Storage.run_sstore_u256 storage (Z.to_nat slot) value)
+  end.
+
+Ltac apply_run_sload_map_u256 :=
+  match goal with
+  | |- {{? _, _, Some (make_state _ _ _ ?storage) |
+      Stdlib.sload (keccak256_tuple2 ?key ?index) ⇓ _
+    | _ ?}} =>
+    eapply (Storage.run_sload_map_u256 storage (Z.to_nat index) _ key);
+    try reflexivity
+  end.
+
+Ltac apply_run_sstore_map_u256 :=
+  match goal with
+  | |- {{? _, _, Some (make_state _ _ _ ?storage) |
+      Stdlib.sstore (keccak256_tuple2 ?key ?index) ?value ⇓ _
+    | _ ?}} =>
+    eapply (Storage.run_sstore_map_u256 storage (Z.to_nat index) key value);
+    try reflexivity;
+    try apply State.get_current_storage_with_current_storage_eq
+  end.
+
+Ltac apply_run_sload_map2_u256 :=
+  match goal with
+  | |- {{? _, _, Some (make_state _ _ _ ?storage) |
+      Stdlib.sload (keccak256_tuple2 ?key2 (keccak256_tuple2 ?key1 ?index)) ⇓ _
+    | _ ?}} =>
+    eapply (Storage.run_sload_map2_u256 storage (Z.to_nat index) _ key1 key2);
+    try reflexivity
+  end.
+
+Ltac apply_run_sstore_map2_u256 :=
+  match goal with
+  | |- {{? _, _, Some (make_state _ _ _ ?storage) |
+      Stdlib.sstore (keccak256_tuple2 ?key2 (keccak256_tuple2 ?key1 ?index)) ?value ⇓ _
+    | _ ?}} =>
+    eapply (Storage.run_sstore_map2_u256 storage (Z.to_nat index) key1 key2 value);
+    try reflexivity;
+    try apply State.get_current_storage_with_current_storage_eq
+  end.
+
+Ltac apply_run_keccak256_tuple2 :=
+  match goal with
+  | |- {{? _, _, Some (make_state _ _ ?memory _) | Stdlib.keccak256 ?pointer 64 ⇓ _ | _ ?}} =>
+    apply (run_keccak256_tuple2 _ _ _ memory (Z.to_nat (pointer / 32)));
+    try reflexivity;
+    try apply get_memory_make_state_eq
+  end.
